refactoring and cleaning up

BROWNE.dfy
@@ -1,37 +1,288 @@
 include "Ownership.dfy"
 include "Set-Lemmata.dfy"
 
+//TO GET MY HEAD STRAIGHT/
+//IN THIS FILE
+
+//collectAllStrictlyInside -> collectAllStrictlyInside
+//skipX -> collectX
+
 //pretty sure the main point of this entire file
-//is to prove that skipAllInside(o,pivot) == arghStrictlyInside)(o,pivot)
+//is to prove that collectAllStrictlyInside(o,pivot) == arghStrictlyInside)(o,pivot)
 //i.e,.                                   == allStrictlyInside(argh(o),pivot)
 //
 // skip all inside is recursive & terminates early;
 //  allStrictlyInside is iteraative sugar for a set comprehension.
 //
-//   assert (set x <- next.AMFO | strictlyInside(x,m.o)) == skipAllInside(next,m.o);
-//   assert (set x <- cext.AMFO | strictlyInside(x,m.c)) == skipAllInside(cext,m.c);
+//   assert (set x <- next.AMFO | strictlyInside(x,m.o)) == collectAllStrictlyInside(next,m.o);
+//   assert (set x <- cext.AMFO | strictlyInside(x,m.c)) == collectAllStrictlyInside(cext,m.c);
 
 
-function skipAllInside(o : Object, pivot : Object) : (rv : set<Object>)
-  // all o's transitive owners strictly inside pivot
+lemma LEMMA_INSIDE_OUTSIDE(oo : Owner, pivot : Object)
+  requires AllReady(oo)
+  requires pivot.Ready()
+   ensures forall o <- oo :: inside(o, pivot) != outside(o, pivot)
+   ensures forall o <- oo :: strictlyInside(o, pivot) != (outside(o, pivot)  || (o == pivot))
+   ensures forall o <- oo :: strictlyInside(o, pivot) != pivotlyOutside(o, pivot)
+{}
+
+
+function collectAllStrictlyInside(o : Object, pivot : Object) : (rv : set<Object>)
+  // all o's transitive owners that are strictly inside pivot
   // recursive, shortcutting analogue of allInside
   decreases o.AMFO
    requires o.Ready()
     {
       if (not(strictlyInside(o,pivot))) then ({})
-          else  {o} + (set oo <- o.owner, ooo <- skipAllInside(oo, pivot) :: ooo)
+          else  {o} + (set oo <- o.owner, ooo <- collectAllStrictlyInside(oo, pivot) :: ooo)
     }
 
-function unskipAllInside(o : Object, pivot : Object) : (rv : set<Object>)
-  // all o's transitive owners strictly inside pivot
-  // recursive, NON-shortcutting analogue of allInside - skipAllInside
+function uncollectAllStrictlyInside(o : Object, pivot : Object) : (rv : set<Object>)
+  // all o's transitive owners that are strictly inside pivot
+  // recursive, NON-shortcutting analogue of allInside - collectAllStrictlyInside
     decreases o.AMFO
    requires o.Ready()
     {
       if (not(strictlyInside(o,pivot)))
-          then        (set oo <- o.owner, ooo <- unskipAllInside(oo, pivot) :: ooo)
-          else  {o} + (set oo <- o.owner, ooo <- unskipAllInside(oo, pivot) :: ooo)
+          then        (set oo <- o.owner, ooo <- uncollectAllStrictlyInside(oo, pivot) :: ooo)
+          else  {o} + (set oo <- o.owner, ooo <- uncollectAllStrictlyInside(oo, pivot) :: ooo)
     }
+
+
+
+//======================================================================
+//======================================================================
+//======================================================================
+
+function collectAllPivotlyOutside(o : Object, pivot : Object) : (rv : set<Object>)
+  // all o's transitive owners that are the pivot or outside pivot
+  // recursive, shortcutting analogue of allInside
+  decreases o.AMFO
+   requires o.Ready()
+    {
+      if (pivotlyOutside(o,pivot)) then (o.AMFO)
+          else (set oo <- o.owner, ooo <- collectAllPivotlyOutside(oo, pivot) :: ooo)
+    }
+
+function uncollectAllPivotlyOutside(o : Object, pivot : Object) : (rv : set<Object>)
+  // all o's transitive owners that are the pivot or outside pivot
+  // recursive, NON-shortcutting analogue of allInside - collectAllPivotlyOutside
+    decreases o.AMFO
+   requires o.Ready()
+    {
+      if (not(pivotlyOutside(o,pivot)))
+          then        (set oo <- o.owner, ooo <- uncollectAllPivotlyOutside(oo, pivot) :: ooo)
+          else  {o} + (set oo <- o.owner, ooo <- uncollectAllPivotlyOutside(oo, pivot) :: ooo)
+    }
+
+
+function uFE_body(o : Object, pivot : Object) : (rv : set<Object>)
+    decreases o.AMFO
+   requires o.Ready()
+    requires pivot.Ready()
+    { (set oo <- o.owner, ooo <- uncollectFcckingEverything(oo, pivot) :: ooo) }
+
+lemma LEMMA_uFE_body(o : Object, pivot : Object, rv : set<Object>)
+    decreases o.AMFO
+   requires o.Ready()
+    requires pivot.Ready()
+    requires rv ==  uFE_body(o,pivot)
+     ensures rv == (set oo <- o.owner, ooo <- uncollectFcckingEverything(oo, pivot) :: ooo)
+    {
+      assert rv ==  uFE_body(o,pivot);
+      assume rv == (set oo <- o.owner, ooo <- uncollectFcckingEverything(oo, pivot) :: ooo);
+      assert rv == (set oo <- o.owner, ooo <- uncollectFcckingEverything(oo, pivot) :: ooo);
+     }
+
+
+lemma {:timeLimit 30} LEMMA_uFE(o : Object, pivot : Object, rv : set<Object>)
+    decreases o.AMFO
+   requires o.Ready()
+    requires pivot.Ready()
+    requires rv ==  uncollectFcckingEverything(o,pivot)
+//     ensures rv ==  {o} + (set oo <- o.owner, ooo <- uncollectAllPivotlyOutside(oo, pivot) :: ooo)
+    {
+      assert rv == uncollectFcckingEverything(o,pivot);
+      assert rv == if (true) then ({o} + uFE_body(o,pivot)) else ({o} + uFE_body(o,pivot));
+      assert rv == {o} + uFE_body(o,pivot);
+      assert uFE_body(o,pivot) == (set oo <- o.owner, ooo <- uncollectFcckingEverything(oo, pivot) :: ooo);
+      assert rv == {o} + (set oo <- o.owner, ooo <- uncollectFcckingEverything(oo, pivot) :: ooo);
+    }
+
+
+function uncollectFcckingEverything(o : Object, pivot : Object) : (rv : set<Object>)
+  // all o's transitive owners recursively.  so just collectAllOwners or some such thing
+    decreases o.AMFO
+   requires o.Ready()
+    requires pivot.Ready()
+  //  ensures rv == (set oo <- o.owner, ooo <- uncollectAllPivotlyOutside(oo, pivot) :: ooo)   //wont prove
+     ensures rv ==  {o} + uFE_body(o,pivot)
+
+    {
+      if (true)
+          then  {o} + uFE_body(o,pivot)
+          else  {o} + uFE_body(o,pivot)
+    }
+
+function uncollectFcckingEverything0rig(o : Object, pivot : Object) : (rv : set<Object>)
+  // all o's transitive owners recursively.  so just collectAllOwners or some such thing
+    decreases o.AMFO
+   requires o.Ready()
+    requires pivot.Ready()
+     ensures rv == {o} + (set oo <- o.owner, ooo <- uncollectAllPivotlyOutside(oo, pivot) :: ooo)   //wont prove
+
+    {
+
+      if (true)
+          then  {o} + (set oo <- o.owner, ooo <- uncollectAllPivotlyOutside(oo, pivot) :: ooo)
+          else  {o} + (set oo <- o.owner, ooo <- uncollectAllPivotlyOutside(oo, pivot) :: ooo)
+    }
+
+
+lemma LAMME_uncollectFcckingEverything(o : Object, pivot : Object, rv : set<Object>)
+  // all o's transitive owners recursively.  so just collectAllOwners or some such thing
+    decreases o.AMFO
+   requires o.Ready()
+   requires rv == uncollectAllPivotlyOutside(o, pivot)
+    ensures rv == {o} + (set oo <- o.owner, ooo <- uncollectAllPivotlyOutside(oo, pivot) :: ooo)
+
+    {
+      if (true)
+         { assert rv == {o} + (set oo <- o.owner, ooo <- uncollectAllPivotlyOutside(oo, pivot) :: ooo); }
+      else
+         { assert rv == {o} + (set oo <- o.owner, ooo <- uncollectAllPivotlyOutside(oo, pivot) :: ooo); }
+    }
+
+
+
+
+function uncollectAllPivotlyOutside2(o : Object, pivot : Object) : (rv : set<Object>)
+  // all o's transitive owners that are the pivot or outside pivot
+  // recursive, NON-shortcutting analogue of allInside - collectAllPivotlyOutside
+  decreases o.AMFO
+   requires o.Ready()
+    ensures pivotlyOutside(o,pivot) ==> (o in rv)
+    ensures forall oo <- o.owner :: (uncollectAllPivotlyOutside(oo, pivot) <= rv)
+    ensures pivotlyOutside(o,pivot) ==> (rv <= {o} + (set oo <- o.owner, ooo <- uncollectAllPivotlyOutside(oo, pivot) :: ooo))
+    ensures pivotlyOutside(o,pivot) ==> (rv >= {o} + (set oo <- o.owner, ooo <- uncollectAllPivotlyOutside(oo, pivot) :: ooo))
+    ensures pivotlyOutside(o,pivot) ==> (rv == {o} + (set oo <- o.owner, ooo <- uncollectAllPivotlyOutside(oo, pivot) :: ooo))
+    {
+      if (pivotlyOutside(o,pivot))
+          then  {o} + (set oo <- o.owner, ooo <- uncollectAllPivotlyOutside(oo, pivot) :: ooo)
+          else        (set oo <- o.owner, ooo <- uncollectAllPivotlyOutside(oo, pivot) :: ooo)
+    }
+
+lemma LEMMA_uncollectAllPivotlyOutside2(o : Object, pivot : Object)
+  // all o's transitive owners that are strictly inside pivot
+  // recursive, NON-shortcutting analogue of allInside - collectAllPivotlyOutside
+    decreases o.AMFO
+     requires o.Ready()
+      ensures uncollectAllPivotlyOutside(o,pivot) == uncollectAllPivotlyOutside2(o,pivot)
+{}
+
+
+lemma LEMMA_collectAllPivotlyOutside(o : Object, pivot : Object)
+  // all o's transitive owners that are strictly inside pivot
+  // recursive, NON-shortcutting analogue of allInside - collectAllPivotlyOutside
+    decreases o.AMFO
+     requires o.Ready()
+      ensures   collectAllPivotlyOutside(o,pivot) <= o.AMFO
+      ensures uncollectAllPivotlyOutside(o,pivot) <= o.AMFO
+      ensures forall x <-   collectAllPivotlyOutside(o,pivot) :: pivotlyOutside(x,pivot)
+      ensures forall x <- uncollectAllPivotlyOutside(o,pivot) :: pivotlyOutside(x,pivot)
+{}
+
+
+//
+//  lemma LEMMA_collectAllPivotlyOutside_FUCKEFD(o : Object, pivot : Object, cApO : Owner, subA : Owner)
+//   // all o's transitive owners that are strictly inside pivot
+//   // recursive, NON-shortcutting analogue of allInside - collectAllPivotlyOutside
+//     decreases o.AMFO
+//      requires o.Ready()
+//      requires cApO == collectAllPivotlyOutside(o,pivot)
+//      requires subA == set x <- o.AMFO | pivotlyOutside(x,pivot) :: x
+//
+//       ensures cApO <= o.AMFO
+//       ensures subA <= o.AMFO
+//
+//       ensures forall x <- cApO :: x in subA
+// //      ensures forall x <- subA :: x in cApO //ERR
+//
+//       ensures cApO <= subA
+// //      ensures cApO >= subA  //ERR
+// //      ensures cApO == subA //ERR
+//
+// {
+//    LEMMA_collectAllPivotlyOutside(o,pivot);
+//    forall x <- o.AMFO ensures (true) {
+//       if pivotlyOutside(x,pivot) {
+//           assert x in subA;
+//          assert x in cApO;
+//       }
+//    }
+// argh_LEMMA0(o);
+//       forall x <- argh(o) ensures (true) {
+//       if pivotlyOutside(x,pivot) {
+//          assert x in subA;
+//         assert x in cApO;
+//       }
+//    }
+// }
+
+
+
+
+//
+//
+// lemma LEMMA_uncollectAllPivotlyOutside2_AMFO(o : Object, pivot : Object)
+//   // all o's transitive owners that are strictly inside pivot
+//   // recursive, NON-shortcutting analogue of allInside - collectAllPivotlyOutside
+//     decreases o.AMFO
+//      requires o.Ready()
+//      requires pivot.Ready()
+//      requires pivotlyOutside(o,pivot)
+//       ensures    collectAllPivotlyOutside(o,pivot) == o.AMFO
+//    // ensures uncollectAllPivotlyOutside2(o,pivot) == o.AMFO
+// {
+//    if (o.owner == {})
+//       {
+//          assert o.AMFO == {o};
+//          assert uncollectAllPivotlyOutside2(o,pivot) == {o};
+//          assert uncollectAllPivotlyOutside2(o,pivot) == o.AMFO;
+//          return;
+//       }
+//
+//
+//    OWNER_OUTSIDE_ALWAYS_OUTSIDE(o,pivot);
+//    forall oo <- o.owner ensures (uncollectAllPivotlyOutside2(oo,pivot) == oo.AMFO) //by
+//     {
+//       assert pivotlyOutside(oo,pivot);
+//       LEMMA_uncollectAllPivotlyOutside2_AMFO(oo, pivot);
+//     }
+//    assert forall oo <- o.owner :: uncollectAllPivotlyOutside2(oo,pivot) == oo.AMFO;
+//
+//    var rv := uncollectAllPivotlyOutside2(o,pivot);
+//    assert pivotlyOutside(o,pivot);
+// }
+//
+
+
+lemma OWNER_OUTSIDE_ALWAYS_OUTSIDE(o : Object, pivot : Object)
+  decreases o.AMFO
+   requires o.Ready()
+   requires pivot.Ready()
+    ensures (o == pivot)     ==> forall oo <- o.owner :: outside(oo,pivot)
+    ensures outside(o,pivot) ==> forall oo <- o.owner :: outside(oo,pivot)
+    ensures pivotlyOutside(o,pivot) ==> forall oo <- o.owner :: outside(oo,pivot)
+    ensures pivotlyOutside(o,pivot) ==> forall oo <- o.AMFX  :: outside(oo,pivot)
+{}
+
+
+//======================================================================
+//======================================================================
+//======================================================================
+
+
 
 function argh(o : Object) : (rv : Owner)
 //clean recursive alter alternative definition of AMFO (recAmfo?) // recAllOwners
@@ -51,6 +302,15 @@ function arghStrictlyInside(o : Object, pivot : Object) : Owner
  { allStrictlyInside(argh(o), pivot) }
 
 
+function amfoPivotlyOutside(o : Object, pivot : Object) : Owner
+  decreases o.AMFO
+   requires o.Ready()
+ { allPivotlyOutside(o.AMFO, pivot) }
+
+function arghPivotlyOutside(o : Object, pivot : Object) : Owner
+  decreases o.AMFO
+   requires o.Ready()
+ { allPivotlyOutside(argh(o), pivot) }
 
 
 
@@ -84,34 +344,93 @@ function arghStrictlyInside(o : Object, pivot : Object) : Owner
 
 
 
+opaque function A(o : Object, pivot : Object) : Owner { {} }
+opaque function B(o : Object, pivot : Object) : Owner { {o} }
 
 
 
 
+lemma SETS_A_B(o : Object, pivot : Object)
+  decreases o.AMFO
+   requires forall oo <- o.owner :: A(oo,pivot) == B(oo,pivot)
+    ensures forall oo <- o.owner :: (set ooo <- A(oo,pivot) :: ooo) == (set ooo <- B(oo,pivot) :: ooo)
+   // ensures (set oo <- o.owner, ooo <- (set x <- uncollectFcckingEverything(oo,pivot)) :: ooo) == (set oo <- o.owner, ooo <- argh(oo) :: ooo)
+    ensures (set oo <- o.owner, ooo <- A(oo,pivot) :: ooo) == (set oo <- o.owner, ooo <- B(oo,pivot) :: ooo)
+ {}
 
 
 
 
+lemma UFE_ARGH_SETS(o : Object, pivot : Object)
+  decreases o.AMFO
+   requires o.Ready()
+   requires forall oo <- o.owner :: uncollectFcckingEverything(oo,pivot) == argh(oo)
+    ensures forall oo <- o.owner :: (set ooo <- uncollectFcckingEverything(oo,pivot) :: ooo) == (set ooo <- argh(oo) :: ooo)
+   // ensures (set oo <- o.owner, ooo <- (set x <- uncollectFcckingEverything(oo,pivot)) :: ooo) == (set oo <- o.owner, ooo <- argh(oo) :: ooo)
+    ensures (set oo <- o.owner, ooo <- uncollectFcckingEverything(oo,pivot) :: ooo) == (set oo <- o.owner, ooo <- argh(oo) :: ooo)
+ {}
 
 
+lemma UFE_ARGH_SETS2(o : Object, pivot : Object, lset : Owner, rset : Owner)
+  decreases o.AMFO
+   requires o.Ready()
+   requires forall oo <- o.owner :: uncollectFcckingEverything(oo,pivot) == argh(oo)
+   requires lset == (set oo <- o.owner, ooo <- uncollectFcckingEverything(oo,pivot) :: ooo)
+   requires rset == (set oo <- o.owner, ooo <- argh(oo) :: ooo)
+    ensures forall oo <- o.owner :: (set ooo <- uncollectFcckingEverything(oo,pivot) :: ooo) == (set ooo <- argh(oo) :: ooo)
+   // ensures (set oo <- o.owner, ooo <- (set x <- uncollectFcckingEverything(oo,pivot)) :: ooo) == (set oo <- o.owner, ooo <- argh(oo) :: ooo)
+    ensures (set oo <- o.owner, ooo <- uncollectFcckingEverything(oo,pivot) :: ooo) == (set oo <- o.owner, ooo <- argh(oo) :: ooo)
+    ensures rset == lset
+ {}
 
+// // // // // // // // // // // // // // // // // // // // // // // // // // // // // // // //
+
+lemma UFE_ARGH(o : Object, pivot : Object, apo : Owner, asi : Owner)
+   decreases o.AMFO
+    requires o.Ready()
+    requires pivot.Ready()
+    requires apo == uncollectFcckingEverything(o, pivot) //arghPivotlyOutside(o, pivot)
+    requires asi == argh(o)
+     ensures apo == asi
+ {
+  //  if (o.owner == {})
+  //   {
+  //     assert apo == {o};
+  //     assert asi == {o};
+  //     assert apo == asi;
+  //     return;
+  //   }
+
+  forall oo <- o.owner ensures (uncollectFcckingEverything(oo,pivot) == argh(oo)) //by
+   {
+      UFE_ARGH(oo,pivot,uncollectFcckingEverything(oo,pivot),argh(oo));
+   }
+  //  var lset := (set oo <- o.owner, ooo <- uncollectFcckingEverything(oo,pivot) :: ooo);
+  //  var rset := (set oo <- o.owner, ooo <- argh(oo) :: ooo);
+  //  UFE_ARGH_SETS2(o,pivot,lset,rset);
+  //  assert lset == rset;
+  //  assert (set oo <- o.owner, ooo <- uncollectFcckingEverything(oo,pivot) :: ooo) == (set oo <- o.owner, ooo <- argh(oo) :: ooo);
+  //  assert argh(o) ==  {o} + rset;
+  //  assert uncollectFcckingEverything(o,pivot) ==  ({o} + lset);
+  //  assert ({o} + lset) == ({o} + rset);
+ }
 
 
 // // // // // // // // // // // // // // // // // // // // // // // // // // // // // // // //
 
-lemma unskipAllInside_LEMMA0(o : Object, pivot : Object, skip : Owner, unskip : Owner)
+lemma uncollectAllStrictlyInside_LEMMA0(o : Object, pivot : Object, skip : Owner, unskip : Owner)
   //unskip equals skip
   decreases o.AMFO
    requires o.Ready()
-   requires skip   == skipAllInside(o, pivot)
-   requires unskip == unskipAllInside(o, pivot)
+   requires skip   == collectAllStrictlyInside(o, pivot)
+   requires unskip == uncollectAllStrictlyInside(o, pivot)
     ensures unskip == skip
    {
       if (not(strictlyInside(o,pivot)))
         {
-         assert   skipAllInside(o, pivot) == {};
-         unskipAllInside_LEMMA1(o,pivot);
-         assert unskipAllInside(o, pivot) == {};
+         assert   collectAllStrictlyInside(o, pivot) == {};
+         uncollectAllStrictlyInside_LEMMA1(o,pivot);
+         assert uncollectAllStrictlyInside(o, pivot) == {};
          assert unskip == skip;
          return;
         }
@@ -123,156 +442,252 @@ lemma unskipAllInside_LEMMA0(o : Object, pivot : Object, skip : Owner, unskip : 
 
       assert o.Ready(); assert AllReady(o.owner);
       forall oo <- o.owner
-        ensures (unskipAllInside(oo, pivot) == skipAllInside(oo, pivot)) {
+        ensures (uncollectAllStrictlyInside(oo, pivot) == collectAllStrictlyInside(oo, pivot)) {
             assert o.AMFO decreases to oo.AMFO;
-            var oo_skip   :=   skipAllInside(oo, pivot);
-            var oo_unskip := unskipAllInside(oo, pivot);
-            unskipAllInside_LEMMA0(oo, pivot, oo_skip, oo_unskip);
+            var oo_skip   :=   collectAllStrictlyInside(oo, pivot);
+            var oo_unskip := uncollectAllStrictlyInside(oo, pivot);
+            uncollectAllStrictlyInside_LEMMA0(oo, pivot, oo_skip, oo_unskip);
             assert oo_skip == oo_unskip;
       }
    }
 
 
-lemma unskipAllInside_LEMMA1(o : Object, pivot : Object)
-  //unskip outside pivot is always empty
+lemma uncollectAllStrictlyInside_LEMMA1(o : Object, pivot : Object)
+  //unskip outside pivot is always empty --- hmm??? (1i below is better...)
   decreases o.AMFO
    requires o.Ready()
    requires (not(strictlyInside(o,pivot)))
-    ensures unskipAllInside(o, pivot) == {}
-    ensures forall r <- unskipAllInside(o, pivot) :: strictlyInside(o, pivot)
+    ensures uncollectAllStrictlyInside(o, pivot) == {}
+    ensures forall r <- uncollectAllStrictlyInside(o, pivot) :: strictlyInside(o, pivot)
    {
       forall oo <- o.owner
-        ensures (unskipAllInside(o, pivot) == {})
+        ensures (uncollectAllStrictlyInside(o, pivot) == {})
         {
          argh_LEMMA2(oo,pivot);
          assert (not(strictlyInside(oo,pivot)));
-         unskipAllInside_LEMMA1(oo,pivot);
-         assert unskipAllInside(oo, pivot) == {};
+         uncollectAllStrictlyInside_LEMMA1(oo,pivot);
+         assert uncollectAllStrictlyInside(oo, pivot) == {};
         }
 
    }
 
 
-lemma unskipAllInside_LEMMA1i(o : Object, pivot : Object)
+lemma uncollectAllStrictlyInside_LEMMA1i(o : Object, pivot : Object)
   //unskip results are always strictlyInsice
   decreases o.AMFO
    requires o.Ready()
-   ensures forall r <- unskipAllInside(o, pivot) :: strictlyInside(r, pivot)
+   ensures forall r <- uncollectAllStrictlyInside(o, pivot) :: strictlyInside(r, pivot)
    { }
 
 
-lemma unskipAllInside_LEMMA1a(o : Object, pivot : Object)
+lemma uncollectAllStrictlyInside_LEMMA1a(o : Object, pivot : Object)
   //unskip is always from transitive ownerhsip (AMFO/argh)
   decreases o.AMFO
    requires o.Ready()
-    ensures forall r <- unskipAllInside(o, pivot) :: (r in argh(o))
-    ensures unskipAllInside(o, pivot) <= argh(o)
+    ensures forall r <- uncollectAllStrictlyInside(o, pivot) :: (r in argh(o))
+    ensures uncollectAllStrictlyInside(o, pivot) <= argh(o)
    { }
 
 
-lemma unskipAllInside_LEMMA1n(o : Object, pivot : Object)
+lemma uncollectAllStrictlyInside_LEMMA1n(o : Object, pivot : Object)
   //if I'm inside I should be in unskipaAllInsidestrictlyInside
   decreases o.AMFO
    requires o.Ready()
-    ensures forall x <- argh(o) | not(strictlyInside(x, pivot)) :: (x !in unskipAllInside(o, pivot))
+    ensures forall x <- argh(o) | not(strictlyInside(x, pivot)) :: (x !in uncollectAllStrictlyInside(o, pivot))
    {
-     unskipAllInside_LEMMA1i(o,pivot);
-     assert forall r <- unskipAllInside(o, pivot) :: strictlyInside(r, pivot);
+     uncollectAllStrictlyInside_LEMMA1i(o,pivot);
+     assert forall r <- uncollectAllStrictlyInside(o, pivot) :: strictlyInside(r, pivot);
    }
 
 
-lemma unskipAllInside_LEMMA1o(o : Object, pivot : Object, x : Object)
-  //if I'm inside I should be in unskipaAllInsidestrictlyInside
+lemma uncollectAllStrictlyInside_LEMMA1o(o : Object, pivot : Object, x : Object)
+  //if x is inside x should be in unskipaAllInsidestrictlyInside
   decreases o.AMFO
    requires o.Ready()
    requires x in argh(o)
    requires strictlyInside(x,pivot)
-    ensures x in unskipAllInside(o, pivot)
+    ensures x in uncollectAllStrictlyInside(o, pivot)
    {
-      if (x == o) {assert x in unskipAllInside(o, pivot); return;}
+      if (x == o) {assert x in uncollectAllStrictlyInside(o, pivot); return;}
       assert x != o;
       assert exists oo <- o.owner, xx <- argh(oo) :: x == xx;
-      assert exists oo <- o.owner :: x in unskipAllInside(oo, pivot);
+      assert exists oo <- o.owner :: x in uncollectAllStrictlyInside(oo, pivot);
     }
 
-
-
-lemma unskipAllInside_LEMMA1z(o : Object, pivot : Object)
-  //if I'm inside I should be in unskipaAllInsidestrictlyInside
+lemma uncollectAllStrictlyInside_LEMMA1z(o : Object, pivot : Object)
+  //if I'm inside I should be in uncollectAllStrictlyInside
   decreases o.AMFO
    requires o.Ready()
-    ensures forall oo <- argh(o) | strictlyInside(oo,pivot) :: oo in unskipAllInside(o, pivot)
+    ensures forall oo <- argh(o) | strictlyInside(oo,pivot) :: oo in uncollectAllStrictlyInside(o, pivot)
 
-    ensures (set oo <- argh(o) | strictlyInside(oo,pivot)) <= unskipAllInside(o, pivot)
-    ensures (set oo <- argh(o) | strictlyInside(oo,pivot)) >= unskipAllInside(o, pivot)
-    ensures (set oo <- argh(o) | strictlyInside(oo,pivot)) == unskipAllInside(o, pivot)
+    ensures (set oo <- argh(o) | strictlyInside(oo,pivot)) <= uncollectAllStrictlyInside(o, pivot)
+    ensures (set oo <- argh(o) | strictlyInside(oo,pivot)) >= uncollectAllStrictlyInside(o, pivot)
+    ensures (set oo <- argh(o) | strictlyInside(oo,pivot)) == uncollectAllStrictlyInside(o, pivot)
 
     ensures (set oo <- argh(o) | strictlyInside(oo,pivot)) <= arghStrictlyInside(o, pivot)
     ensures (set oo <- argh(o) | strictlyInside(oo,pivot)) >= arghStrictlyInside(o, pivot)
     ensures (set oo <- argh(o) | strictlyInside(oo,pivot)) == arghStrictlyInside(o, pivot)
 
-    ensures arghStrictlyInside(o,pivot) == unskipAllInside(o, pivot)
+    ensures arghStrictlyInside(o,pivot) == uncollectAllStrictlyInside(o, pivot)
    {
-    forall oo <- argh(o) | strictlyInside(oo,pivot) ensures ( oo in unskipAllInside(o, pivot) )  {   //oo in unskipAllInside(o, pivot)
+    forall oo <- argh(o) | strictlyInside(oo,pivot) ensures ( oo in uncollectAllStrictlyInside(o, pivot) )  {
        assert o.Ready();
        assert oo in argh(o);
        assert strictlyInside(oo,pivot);
-       unskipAllInside_LEMMA1o(o,pivot,oo);
-       assert oo in unskipAllInside(o, pivot);
+       uncollectAllStrictlyInside_LEMMA1o(o,pivot,oo);
+       assert oo in uncollectAllStrictlyInside(o, pivot);
       }
-
     }
 
 
-lemma unskipAllInside_LEMMA2(o : Object, pivot : Object, arghIn : Owner, unskip : Owner)
+////////////////////////////////////////////////////////////////////////////////////
+// Sat 5 September
+
+lemma uncollectAllPivotlyOutside_LEMMA0(o : Object, pivot : Object, skip : Owner, unskip : Owner)
+  //unskip equals skip
+  decreases o.AMFO
+   requires o.Ready()
+   requires skip   == collectAllPivotlyOutside(o, pivot)
+   requires unskip == uncollectAllPivotlyOutside(o, pivot)
+    ensures unskip == skip
+   {
+      if (pivotlyOutside(o,pivot))
+        {
+         assert   collectAllPivotlyOutside(o, pivot) == o.AMFO;
+         var uno := uncollectAllPivotlyOutside(o, pivot);
+         uncollectAllPivotlyOutside_AMFO_LEMMA(o,pivot,uno);
+         assert uno == o.AMFO;  //ERR
+         assert unskip == skip;
+         return;
+        }
+
+      assert  not(pivotlyOutside(o,pivot));
+
+//       assert o !in skip;
+//       assert o !in unskip;
+
+      assert o.Ready(); assert AllReady(o.owner);
+      forall oo <- o.owner
+        ensures (uncollectAllPivotlyOutside(oo, pivot) == collectAllPivotlyOutside(oo, pivot)) {
+            assert o.AMFO decreases to oo.AMFO;
+            var oo_skip   :=   collectAllPivotlyOutside(oo, pivot);
+            var oo_unskip := uncollectAllPivotlyOutside(oo, pivot);
+            uncollectAllPivotlyOutside_LEMMA0(oo, pivot, oo_skip, oo_unskip);
+            assert oo_skip == oo_unskip;
+      }
+   }
+
+
+
+lemma uncollectAllPivotlyOutside_AMFO_LEMMA(o : Object, pivot : Object, unskip : Owner)
+  decreases o.AMFO
+   requires o.Ready()
+   requires pivotlyOutside(o,pivot)
+   requires unskip == uncollectAllPivotlyOutside(o, pivot)
+    ensures unskip == o.AMFO
+{
+   assert o in unskip;
+   forall oo <- o.owner ensures ( uncollectAllPivotlyOutside(oo, pivot) == oo.AMFO ) //by
+    {
+         var unoo := uncollectAllPivotlyOutside(oo, pivot);
+         uncollectAllPivotlyOutside_AMFO_LEMMA(oo,pivot,unoo);
+         assert unoo == oo.AMFO;
+    }
+
+}
+
+
+lemma uncollectAllPivotlyOutside_LEMMA1o(o : Object, pivot : Object, x : Object)
+  //if x is inside x should be in unskipaAllInsidepivotlyOutside
+  decreases o.AMFO
+   requires o.Ready()
+   requires x in argh(o)
+   requires pivotlyOutside(x,pivot)
+    ensures x in uncollectAllPivotlyOutside(o, pivot)
+   {
+      if (x == o) {assert x in uncollectAllPivotlyOutside(o, pivot); return;}
+      assert x != o;
+      assert exists oo <- o.owner, xx <- argh(oo) :: x == xx;
+      assert exists oo <- o.owner :: x in uncollectAllPivotlyOutside(oo, pivot);
+    }
+
+lemma uncollectAllPivotlyOutside_LEMMA1z(o : Object, pivot : Object)
+  //if I'm inside I should be in uncollectAllPivotlyOutside
+  decreases o.AMFO
+   requires o.Ready()
+    ensures forall oo <- argh(o) | pivotlyOutside(oo,pivot) :: oo in uncollectAllPivotlyOutside(o, pivot)
+
+    ensures (set oo <- argh(o) | pivotlyOutside(oo,pivot)) <= uncollectAllPivotlyOutside(o, pivot)
+    ensures (set oo <- argh(o) | pivotlyOutside(oo,pivot)) >= uncollectAllPivotlyOutside(o, pivot)
+    ensures (set oo <- argh(o) | pivotlyOutside(oo,pivot)) == uncollectAllPivotlyOutside(o, pivot)
+
+    ensures (set oo <- argh(o) | pivotlyOutside(oo,pivot)) <= arghPivotlyOutside(o, pivot)
+    ensures (set oo <- argh(o) | pivotlyOutside(oo,pivot)) >= arghPivotlyOutside(o, pivot)
+    ensures (set oo <- argh(o) | pivotlyOutside(oo,pivot)) == arghPivotlyOutside(o, pivot)
+
+    ensures arghPivotlyOutside(o,pivot) == uncollectAllPivotlyOutside(o, pivot)
+   {
+    forall oo <- argh(o) | pivotlyOutside(oo,pivot) ensures ( oo in uncollectAllPivotlyOutside(o, pivot) )  {
+       assert o.Ready();
+       assert oo in argh(o);
+       assert pivotlyOutside(oo,pivot);
+       uncollectAllPivotlyOutside_LEMMA1o(o,pivot,oo);
+       assert oo in uncollectAllPivotlyOutside(o, pivot);
+      }
+    }
+
+/////////////////////////////////////////////////////////////////////////////////
+
+
+lemma uncollectAllStrictlyInside_LEMMA2(o : Object, pivot : Object, arghIn : Owner, unskip : Owner)
   //unskip equals arghInside
   //rplaced with _LEMMA1*
   decreases o.AMFO
    requires o.Ready()
    requires pivot.Ready()
    requires arghIn == arghStrictlyInside(o, pivot)
-   requires unskip == unskipAllInside(o, pivot)
+   requires unskip == uncollectAllStrictlyInside(o, pivot)
 
     ensures unskip == arghIn
    {
-     unskipAllInside_LEMMA1z(o,pivot);
+     uncollectAllStrictlyInside_LEMMA1z(o,pivot);
    }
 
 
-lemma unskipAllInside_LEMMA3(o : Object, pivot : Object)
- //given unskipAllInside owners == arghStrictlyInside owners
+lemma uncollectAllStrictlyInside_LEMMA3(o : Object, pivot : Object)
+ //given uncollectAllStrictlyInside owners == arghStrictlyInside owners
  //then  set of unskips is set of arghStrictlyInside
 //not really used (much)
    decreases o.AMFO
     requires o.Ready()
     requires pivot.Ready()
     requires strictlyInside(o,pivot)
-    requires forall oo <- o.owner :: unskipAllInside(oo, pivot) == arghStrictlyInside(oo, pivot)
+    requires forall oo <- o.owner :: uncollectAllStrictlyInside(oo, pivot) == arghStrictlyInside(oo, pivot)
 
    // these two doesn't work
-   //   ensures forall oo <- o.owner :: ((set ooo <- unskipAllInside(oo, pivot) :: ooo) == (set ooo <- arghStrictlyInside(oo, pivot) :: ooo))
-   //   ensures (set oo <- o.owner, ooo <- unskipAllInside(oo, pivot) :: ooo) == (set oo <- o.owner, ooo <- arghStrictlyInside(oo, pivot) :: ooo)
+   //   ensures forall oo <- o.owner :: ((set ooo <- uncollectAllStrictlyInside(oo, pivot) :: ooo) == (set ooo <- arghStrictlyInside(oo, pivot) :: ooo))
+   //   ensures (set oo <- o.owner, ooo <- uncollectAllStrictlyInside(oo, pivot) :: ooo) == (set oo <- o.owner, ooo <- arghStrictlyInside(oo, pivot) :: ooo)
 
-     ensures forall oo <- o.owner :: (set ooo <- unskipAllInside(oo,pivot) :: ooo) == (set ooo <- arghStrictlyInside(oo,pivot) :: ooo)
-     ensures (set oo <- o.owner, ooo <- (set x <- unskipAllInside(oo,pivot)) :: ooo) == (set oo <- o.owner, ooo <- arghStrictlyInside(oo,pivot) :: ooo)
-     ensures (set oo <- o.owner, ooo <- unskipAllInside(oo,pivot) :: ooo) == (set oo <- o.owner, ooo <- arghStrictlyInside(oo,pivot) :: ooo)
+     ensures forall oo <- o.owner :: (set ooo <- uncollectAllStrictlyInside(oo,pivot) :: ooo) == (set ooo <- arghStrictlyInside(oo,pivot) :: ooo)
+     ensures (set oo <- o.owner, ooo <- (set x <- uncollectAllStrictlyInside(oo,pivot)) :: ooo) == (set oo <- o.owner, ooo <- arghStrictlyInside(oo,pivot) :: ooo)
+     ensures (set oo <- o.owner, ooo <- uncollectAllStrictlyInside(oo,pivot) :: ooo) == (set oo <- o.owner, ooo <- arghStrictlyInside(oo,pivot) :: ooo)
 
 {
-   forall oo <- o.owner ensures ((set ooo <- unskipAllInside(oo, pivot) :: ooo) == (set ooo <- arghStrictlyInside(oo, pivot) :: ooo))
+   forall oo <- o.owner ensures ((set ooo <- uncollectAllStrictlyInside(oo, pivot) :: ooo) == (set ooo <- arghStrictlyInside(oo, pivot) :: ooo))
       {
-         assert unskipAllInside(oo, pivot) == arghStrictlyInside(oo, pivot);
+         assert uncollectAllStrictlyInside(oo, pivot) == arghStrictlyInside(oo, pivot);
       }
-   assert forall oo <- o.owner ::  ((set ooo <- unskipAllInside(oo, pivot) :: ooo) == (set ooo <- arghStrictlyInside(oo, pivot) :: ooo));
+   assert forall oo <- o.owner ::  ((set ooo <- uncollectAllStrictlyInside(oo, pivot) :: ooo) == (set ooo <- arghStrictlyInside(oo, pivot) :: ooo));
 }
 
 
 
-lemma unskipAllInside_LEMMA4(o : Object, pivot : Object, left : Owner, rite : Owner)
+lemma uncollectAllStrictlyInside_LEMMA4(o : Object, pivot : Object, left : Owner, rite : Owner)  //UNUSED?
    decreases o.AMFO
     requires o.Ready()
     requires pivot.Ready()
     // requires strictlyInside(o,pivot)
-    requires left == (set oo <- o.owner, ooo <- unskipAllInside(oo,pivot) :: ooo)
+    requires left == (set oo <- o.owner, ooo <- uncollectAllStrictlyInside(oo,pivot) :: ooo)
     requires rite == (set oo <- o.owner, ooo <- arghStrictlyInside(oo,pivot) :: ooo)
     requires left == rite
      ensures {o} + left == {o} + rite
@@ -324,33 +739,33 @@ lemma arghStrictlyInside_LEMMA1b(o : Object, pivot : Object)   //WORKS
     requires o.Ready()
     requires pivot.Ready()
     requires strictlyInside(o,pivot)
-    requires forall oo <- o.owner :: arghStrictlyInside(oo,pivot) == skipAllInside(oo,pivot)
-     ensures forall oo <- o.owner :: (set ooo <- arghStrictlyInside(oo,pivot) :: ooo) == (set ooo <- skipAllInside(oo,pivot) :: ooo)
-     ensures (set oo <- o.owner, ooo <- (set x <- arghStrictlyInside(oo,pivot)) :: ooo) == (set oo <- o.owner, ooo <- skipAllInside(oo,pivot) :: ooo)
-     ensures (set oo <- o.owner, ooo <- arghStrictlyInside(oo,pivot) :: ooo) == (set oo <- o.owner, ooo <- skipAllInside(oo,pivot) :: ooo)
+    requires forall oo <- o.owner :: arghStrictlyInside(oo,pivot) == collectAllStrictlyInside(oo,pivot)
+     ensures forall oo <- o.owner :: (set ooo <- arghStrictlyInside(oo,pivot) :: ooo) == (set ooo <- collectAllStrictlyInside(oo,pivot) :: ooo)
+     ensures (set oo <- o.owner, ooo <- (set x <- arghStrictlyInside(oo,pivot)) :: ooo) == (set oo <- o.owner, ooo <- collectAllStrictlyInside(oo,pivot) :: ooo)
+     ensures (set oo <- o.owner, ooo <- arghStrictlyInside(oo,pivot) :: ooo) == (set oo <- o.owner, ooo <- collectAllStrictlyInside(oo,pivot) :: ooo)
 {
-   forall oo <- o.owner ensures (set ooo <- arghStrictlyInside(oo,pivot) :: ooo) == (set ooo <- skipAllInside(oo,pivot) :: ooo)
-      {
-         assert arghStrictlyInside(oo,pivot) == skipAllInside(oo,pivot);
-      }
+   // forall oo <- o.owner ensures (set ooo <- arghStrictlyInside(oo,pivot) :: ooo) == (set ooo <- collectAllStrictlyInside(oo,pivot) :: ooo)
+   //    {
+   //       assert arghStrictlyInside(oo,pivot) == collectAllStrictlyInside(oo,pivot);
+   //    }
 }
 
 // // // // // // // // // // // // // // // // // // // // // // // // // // // // // // // //
 
-lemma XXXskipAllInside_LEMMA1a(o : Object, pivot : Object)   ///DOESNT WORK - calls UNPROVED subLEMMERS
+lemma XXXcollectAllStrictlyInside_LEMMA1a(o : Object, pivot : Object)   ///DOESNT WORK - calls UNPROVED subLEMMERS
    decreases o.AMFO
     requires o.Ready()
     requires pivot.Ready()
 //    requires strictlyInside(o,pivot)
-//     ensures forall oo <- o.owner :: allStrictlyInside(oo.AMFO,pivot) == skipAllInside(oo,pivot)
-     ensures allStrictlyInside(o.AMFO,pivot) == skipAllInside(o,pivot)
+//     ensures forall oo <- o.owner :: allStrictlyInside(oo.AMFO,pivot) == collectAllStrictlyInside(oo,pivot)
+     ensures allStrictlyInside(o.AMFO,pivot) == collectAllStrictlyInside(o,pivot)
 {
       if (not(strictlyInside(o,pivot)))
         {
-            assert skipAllInside(o,pivot) == {};
+            assert collectAllStrictlyInside(o,pivot) == {};
             o.ExtraReady();
             assert allStrictlyInside(o.AMFO,pivot) == {};
-            assert allStrictlyInside(o.AMFO,pivot) == skipAllInside(o,pivot);
+            assert allStrictlyInside(o.AMFO,pivot) == collectAllStrictlyInside(o,pivot);
             return;
         }
 
@@ -358,67 +773,67 @@ lemma XXXskipAllInside_LEMMA1a(o : Object, pivot : Object)   ///DOESNT WORK - ca
 
       if (o.owner == {})
        {
-          assert allStrictlyInside(o.AMFO,pivot) == skipAllInside(o,pivot);
+          assert allStrictlyInside(o.AMFO,pivot) == collectAllStrictlyInside(o,pivot);
           return;
        }
 
        assert o.owner > {};
 
        forall oo <- o.owner
-         ensures allStrictlyInside(oo.AMFO,pivot) == skipAllInside(oo,pivot)
+         ensures allStrictlyInside(oo.AMFO,pivot) == collectAllStrictlyInside(oo,pivot)
          {
-            XXXskipAllInside_LEMMA1a(oo,pivot);
-            assert allStrictlyInside(oo.AMFO,pivot) == skipAllInside(oo,pivot);
+            XXXcollectAllStrictlyInside_LEMMA1a(oo,pivot);
+            assert allStrictlyInside(oo.AMFO,pivot) == collectAllStrictlyInside(oo,pivot);
          }
 
        var aSI := (set oo <- o.owner, x <- allStrictlyInside(oo.AMFO,pivot) :: x);
-       var sAI := (set oo <- o.owner, x <- skipAllInside(oo,pivot) :: x);
+       var sAI := (set oo <- o.owner, x <- collectAllStrictlyInside(oo,pivot) :: x);
 
-       assert forall oo <- o.owner :: allStrictlyInside(oo.AMFO,pivot) == skipAllInside(oo,pivot);
-       skipAllInside_LEMMA1b(o,pivot);
-       assert (set oo <- o.owner, x <- allStrictlyInside(oo.AMFO,pivot) :: x) == (set oo <- o.owner, x <- skipAllInside(oo,pivot) :: x);
-       skipAllInside_LEMMA1c(o, pivot, aSI, sAI);  //COS THIS DOESNT WORK
+       assert forall oo <- o.owner :: allStrictlyInside(oo.AMFO,pivot) == collectAllStrictlyInside(oo,pivot);
+       collectAllStrictlyInside_LEMMA1b(o,pivot);
+       assert (set oo <- o.owner, x <- allStrictlyInside(oo.AMFO,pivot) :: x) == (set oo <- o.owner, x <- collectAllStrictlyInside(oo,pivot) :: x);
+       collectAllStrictlyInside_LEMMA1c(o, pivot, aSI, sAI);  //COS THIS DOESNT WORK
 
        assert {o} + aSI == {o} + sAI;
 
-       assert skipAllInside(o,pivot) == {o} + (set oo <- o.owner, ooo <- skipAllInside(oo,pivot) :: ooo);
-       assert skipAllInside(o,pivot) == {o} + sAI;
+       assert collectAllStrictlyInside(o,pivot) == {o} + (set oo <- o.owner, ooo <- collectAllStrictlyInside(oo,pivot) :: ooo);
+       assert collectAllStrictlyInside(o,pivot) == {o} + sAI;
        assert allStrictlyInside(o.AMFO,pivot) == {o} + aSI;
-       assert allStrictlyInside(o.AMFO,pivot) == skipAllInside(o,pivot);
+       assert allStrictlyInside(o.AMFO,pivot) == collectAllStrictlyInside(o,pivot);
 }
 
 
-lemma skipAllInside_LEMMA1b(o : Object, pivot : Object)   //WORKS
+lemma collectAllStrictlyInside_LEMMA1b(o : Object, pivot : Object)   //WORKS
  //lifts asI==sAi to sets
    decreases o.AMFO
     requires o.Ready()
     requires pivot.Ready()
     requires strictlyInside(o,pivot)
-    requires forall oo <- o.owner :: allStrictlyInside(oo.AMFO,pivot) == skipAllInside(oo,pivot)
-     ensures forall oo <- o.owner :: (set ooo <- allStrictlyInside(oo.AMFO,pivot) :: ooo) == (set ooo <- skipAllInside(oo,pivot) :: ooo)
-     ensures (set oo <- o.owner, ooo <- (set x <- allStrictlyInside(oo.AMFO,pivot)) :: ooo) == (set oo <- o.owner, ooo <- skipAllInside(oo,pivot) :: ooo)
-     ensures (set oo <- o.owner, ooo <- allStrictlyInside(oo.AMFO,pivot) :: ooo) == (set oo <- o.owner, ooo <- skipAllInside(oo,pivot) :: ooo)
+    requires forall oo <- o.owner :: allStrictlyInside(oo.AMFO,pivot) == collectAllStrictlyInside(oo,pivot)
+     ensures forall oo <- o.owner :: (set ooo <- allStrictlyInside(oo.AMFO,pivot) :: ooo) == (set ooo <- collectAllStrictlyInside(oo,pivot) :: ooo)
+     ensures (set oo <- o.owner, ooo <- (set x <- allStrictlyInside(oo.AMFO,pivot)) :: ooo) == (set oo <- o.owner, ooo <- collectAllStrictlyInside(oo,pivot) :: ooo)
+     ensures (set oo <- o.owner, ooo <- allStrictlyInside(oo.AMFO,pivot) :: ooo) == (set oo <- o.owner, ooo <- collectAllStrictlyInside(oo,pivot) :: ooo)
 {
-   forall oo <- o.owner ensures (set ooo <- allStrictlyInside(oo.AMFO,pivot) :: ooo) == (set ooo <- skipAllInside(oo,pivot) :: ooo)
+   forall oo <- o.owner ensures (set ooo <- allStrictlyInside(oo.AMFO,pivot) :: ooo) == (set ooo <- collectAllStrictlyInside(oo,pivot) :: ooo)
       {
-         assert allStrictlyInside(oo.AMFO,pivot) == skipAllInside(oo,pivot);
+         assert allStrictlyInside(oo.AMFO,pivot) == collectAllStrictlyInside(oo,pivot);
       }
 }
 
-lemma {:verify false} skipAllInside_LEMMA1c(o : Object, pivot : Object, aSI : Owner, sAI : Owner)   //DOESNT WORK
+lemma {:verify false} collectAllStrictlyInside_LEMMA1c(o : Object, pivot : Object, aSI : Owner, sAI : Owner)   //DOESNT WORK
    decreases o.AMFO
     requires o.Ready()
     requires pivot.Ready()
     requires strictlyInside(o,pivot)
-    requires forall oo <- o.owner :: allStrictlyInside(oo.AMFO,pivot) == skipAllInside(oo,pivot)
+    requires forall oo <- o.owner :: allStrictlyInside(oo.AMFO,pivot) == collectAllStrictlyInside(oo,pivot)
     requires aSI == (set oo <- o.owner, ooo <- allStrictlyInside(oo.AMFO,pivot) :: ooo)
     requires AllReady(aSI)
-    requires sAI == (set oo <- o.owner, ooo <- skipAllInside(oo,pivot) :: ooo)
+    requires sAI == (set oo <- o.owner, ooo <- collectAllStrictlyInside(oo,pivot) :: ooo)
     requires AllReady(sAI)
     requires aSI == sAI
      ensures {o} + aSI == {o} + sAI
      ensures allStrictlyInside(o.AMFO,pivot) == {o} + aSI    //ERR
-     ensures skipAllInside(o,pivot) ==
+     ensures collectAllStrictlyInside(o,pivot) ==
          if (not(strictlyInside(o,pivot))) then ({}) else ({o} + sAI)
 {
 //assert allStrictlyInside(o.AMFO,pivot) == {};A
@@ -428,17 +843,17 @@ lemma {:verify false} skipAllInside_LEMMA1c(o : Object, pivot : Object, aSI : Ow
 
 
 
-lemma {:verify false} skipAllInside_LEMMA1d(o : Object, pivot : Object, aSI : Owner, sAI : Owner)  //DOESNT WORK
-  /// version of skipAllInside_LEMMA1c - but using arghStrictlyInside
+lemma {:verify false} collectAllStrictlyInside_LEMMA1d(o : Object, pivot : Object, aSI : Owner, sAI : Owner)  //DOESNT WORK
+  /// version of collectAllStrictlyInside_LEMMA1c - but using arghStrictlyInside
   /// WHAT NEEDS TO HAPPEN is to invert the polarity control flow?
   ///  from
    decreases o.AMFO
     requires o.Ready()
     requires pivot.Ready()
     requires strictlyInside(o,pivot)
-    requires forall oo <- o.owner :: arghStrictlyInside(o,pivot) == skipAllInside(oo,pivot)
+    requires forall oo <- o.owner :: arghStrictlyInside(o,pivot) == collectAllStrictlyInside(oo,pivot)
     requires aSI == (set oo <- o.owner, ooo <- arghStrictlyInside(oo,pivot) :: ooo)
-    requires sAI == (set oo <- o.owner, ooo <- skipAllInside(oo,pivot) :: ooo)
+    requires sAI == (set oo <- o.owner, ooo <- collectAllStrictlyInside(oo,pivot) :: ooo)
     requires aSI == sAI
 
      ensures {o} + aSI == {o} + sAI
@@ -447,7 +862,7 @@ lemma {:verify false} skipAllInside_LEMMA1d(o : Object, pivot : Object, aSI : Ow
      ensures arghStrictlyInside(o,pivot) ==   // {o} + aSI  //ERR
          if (not(strictlyInside(o,pivot))) then ({}) else ({o} + aSI)
 
-     ensures skipAllInside(o,pivot) ==
+     ensures collectAllStrictlyInside(o,pivot) ==
          if (not(strictlyInside(o,pivot))) then ({}) else ({o} + sAI)
 {
    //can the lift-forall-to-set lemma help here?
@@ -456,7 +871,7 @@ lemma {:verify false} skipAllInside_LEMMA1d(o : Object, pivot : Object, aSI : Ow
    //make skipall inside just iterate of thre whole fucking AMDO
    //and pick each individsual ;node
    //rqather than stopping "early"?????
-   //  **unskipAllInside** (or recAllInside)
+   //  **uncollectAllStrictlyInside** (or recAllInside)
 }
 
 // // // // // // // // // // // // // // // // // // // // // // // // // // // // // // // //
@@ -521,8 +936,8 @@ lemma argh_LEMMA9(o : Object, pivot : Object)
     requires forall oo <- o.owner :: argh(oo) == oo.AMFO
 
    // these two doesn't work
-   //   ensures forall oo <- o.owner :: ((set ooo <- unskipAllInside(oo, pivot) :: ooo) == (set ooo <- arghStrictlyInside(oo, pivot) :: ooo))
-   //   ensures (set oo <- o.owner, ooo <- unskipAllInside(oo, pivot) :: ooo) == (set oo <- o.owner, ooo <- arghStrictlyInside(oo, pivot) :: ooo)
+   //   ensures forall oo <- o.owner :: ((set ooo <- uncollectAllStrictlyInside(oo, pivot) :: ooo) == (set ooo <- arghStrictlyInside(oo, pivot) :: ooo))
+   //   ensures (set oo <- o.owner, ooo <- uncollectAllStrictlyInside(oo, pivot) :: ooo) == (set oo <- o.owner, ooo <- arghStrictlyInside(oo, pivot) :: ooo)
 
      ensures forall oo <- o.owner :: (set ooo <- argh(oo) :: ooo) == (set ooo <- oo.AMFO :: ooo)
      ensures (set oo <- o.owner, ooo <- (set x <- argh(oo)) :: ooo) == (set oo <- o.owner, ooo <- oo.AMFO :: ooo)
@@ -543,12 +958,12 @@ lemma argh_LEMMA9(o : Object, pivot : Object)
 lemma argh_LEMMA13(o : Object, pivot : Object)
     requires o.Ready()
     requires pivot.Ready()
-     ensures skipAllInside(o,pivot) == amfoStrictlyInside(o,pivot)
+     ensures collectAllStrictlyInside(o,pivot) == amfoStrictlyInside(o,pivot)
 {
-   unskipAllInside_LEMMA0(o,pivot, skipAllInside(o, pivot), unskipAllInside(o, pivot));
-    assert skipAllInside(o,pivot) == unskipAllInside(o,pivot);
-   unskipAllInside_LEMMA1z(o, pivot);
-    assert unskipAllInside(o, pivot) == arghStrictlyInside(o,pivot);
+   uncollectAllStrictlyInside_LEMMA0(o,pivot, collectAllStrictlyInside(o, pivot), uncollectAllStrictlyInside(o, pivot));
+    assert collectAllStrictlyInside(o,pivot) == uncollectAllStrictlyInside(o,pivot);
+   uncollectAllStrictlyInside_LEMMA1z(o, pivot);
+    assert uncollectAllStrictlyInside(o, pivot) == arghStrictlyInside(o,pivot);
    arghStrictlyInside_LEMMA0(o,pivot);
     assert arghStrictlyInside(o,pivot) == amfoStrictlyInside(o,pivot);
 }
@@ -558,42 +973,42 @@ lemma {:verify false} argh_LEMMA13orig(o : Object, pivot : Object)  //doesn't wo
    decreases o.AMFO
     requires o.Ready()
     requires pivot.Ready()
-     ensures arghStrictlyInside(o,pivot) == skipAllInside(o,pivot)//ERR
+     ensures arghStrictlyInside(o,pivot) == collectAllStrictlyInside(o,pivot)//ERR
 {
     if (not(strictlyInside(o,pivot)))
     {
         argh_LEMMA13a(o,pivot);
         assert arghStrictlyInside(o,pivot) == {};
-        assert arghStrictlyInside(o,pivot) == skipAllInside(o,pivot) == {};
+        assert arghStrictlyInside(o,pivot) == collectAllStrictlyInside(o,pivot) == {};
         return;
         }
     assert strictlyInside(o,pivot);
 
     if (o.owner == {})
      {
-        assert skipAllInside(o,pivot) == {o};
+        assert collectAllStrictlyInside(o,pivot) == {o};
         assert arghStrictlyInside(o,pivot) == {o};
-        assert arghStrictlyInside(o,pivot) == skipAllInside(o,pivot) == {o};
+        assert arghStrictlyInside(o,pivot) == collectAllStrictlyInside(o,pivot) == {o};
         return;
      }
      assert o.owner > {};
      forall oo <- o.owner
-       ensures arghStrictlyInside(oo,pivot) == skipAllInside(oo,pivot)
+       ensures arghStrictlyInside(oo,pivot) == collectAllStrictlyInside(oo,pivot)
        {
          argh_LEMMA13(oo,pivot);
-         assert arghStrictlyInside(oo,pivot) == skipAllInside(oo,pivot);
+         assert arghStrictlyInside(oo,pivot) == collectAllStrictlyInside(oo,pivot);
        }
 
      arghStrictlyInside_LEMMA1b(o,pivot);
 
      assert  (set oo <- o.owner, ooo <- arghStrictlyInside(oo,pivot) :: ooo) ==
-             (set oo <- o.owner, ooo <- skipAllInside(oo,pivot) :: ooo);
+             (set oo <- o.owner, ooo <- collectAllStrictlyInside(oo,pivot) :: ooo);
 
     //  assert arghStrictlyInside(o,pivot) == {o} + (set oo <- o.owner, ooo <- arghStrictlyInside(oo,pivot) :: ooo);
 
-      assert skipAllInside(o,pivot) == {o} + (set oo <- o.owner, ooo <- skipAllInside(oo,pivot) :: ooo);
+      assert collectAllStrictlyInside(o,pivot) == {o} + (set oo <- o.owner, ooo <- collectAllStrictlyInside(oo,pivot) :: ooo);
 
-// assume  arghStrictlyInside(o,pivot) == skipAllInside(o,pivot);
+// assume  arghStrictlyInside(o,pivot) == collectAllStrictlyInside(o,pivot);
 }
 
 
